$ \vert E_s \vert = S \sqrt{ \frac{dW \ y_{Rx}}{(1+(\frac{w}{y_{Tx}})^2)^{1/2}}
(y^2_{Rx} + (x_{Rx} - x_{Tx} - w)^2)^{\frac{3}{4}}} $

1. If $ x(t) = \frac{a \pm \sqrt{a^2 + bd}}{b} $, where

\begin{align*}
   a &= [ 2x_s ( 1 + \gamma ) ][ y^2_i - y^2_s - (tc)^2 - x^2_s (1 -\gamma^2 ) ] ] + 4(tc)^2 x_s \\
   b &= 4(tc)^2 - [ 2x_s (1+ \gamma) ]^2 \\
   d &= [ y^2_i - y^2_s - (tc)^2 - x^2_s (1 -\gamma^2 ) ] - 4(tc)^2 x^2_s - 4(tc)^2 y^2_s
\end{align*}

can you simplify the expression for $x$ as much as possible?
A: nothing simple...

2. What if $r_i = \sqrt{y^2_i + (x-x_i)^2} $ and $r_s = \sqrt{y^2_s + (x_s-x)^2}$
